Termination proofs and work on soundness proofs for big-step semantics

hol/symb_exec/p4_bigstepScript.sml
@@ -1,5 +1,5 @@
 open HolKernel boolLib liteLib simpLib Parse bossLib;
-open p4Theory p4_exec_semTheory;
+open p4Theory p4_auxTheory p4_exec_semTheory;
 
 val _ = new_theory "p4_bigstep";
 
@@ -13,7 +13,6 @@ val _ = new_theory "p4_bigstep";
 
 (***********************)
 (*   Main semantics    *)
-
 
 Definition lookup_vexp_def:
  lookup_vexp scope_list x =
@@ -182,7 +181,16 @@ Definition bigstep_e_exec_def:
     | NONE => NONE)
   | NONE => NONE)
 Termination
-cheat
+WF_REL_TAC `measure ( \ t. case t of
+                           | (INL (scope_lists, e, n)) => e_size e
+                           | (INR (scope_lists, e_l, n)) => e3_size e_l)` >>
+fs[e_size_def] >>
+Induct_on ‘x_e_l’ >> (
+ fs[e_size_def]
+) >>
+rpt strip_tac >>
+PairCases_on ‘h’ >>
+fs[e_size_def]
 End
 
 (* TODO: No reduction to L-values, for now *)
@@ -343,9 +351,1335 @@ Definition bigstep_arch_exec'_def:
  (bigstep_arch_exec' _ _ _ = NONE)
 End
 
+val bigstep_e_exec_case_tac =
+ Cases_on ‘bigstep_e_exec scope_lists e'' 0’ >> (
+  fs[]
+ ) >>
+ PairCases_on ‘x’ >>
+ fs[]
+;
+
+val bigstep_e_exec_case'_tac =
+ Cases_on ‘bigstep_e_exec scope_lists e n’ >> (
+  fs[]
+ ) >>
+ PairCases_on ‘x’ >>
+ fs[]
+;
+
+ (* TODO
+val induct_traverse_e_then_tac tac =
+
+;
+*)
+
+Theorem bigstep_e_exec_l_incr:
+!e_l e_l' scope_lists n m.
+bigstep_e_exec_l scope_lists e_l n = SOME (e_l', m) ==>
+n <= m
+Proof
+Induct_on ‘e_l’ >> (
+rpt disch_tac >>
+ fs[bigstep_e_exec_def]
+) >>
+cheat
+(*
+(* OLD *)
+Induct_on ‘h’ >> (
+ fs[bigstep_e_exec_def]
+) >| [
+ rpt strip_tac >>
+ Cases_on ‘bigstep_e_exec_l scope_lists e_l n’ >> (
+  fs[]
+ ) >>
+ PairCases_on ‘x’ >>
+ fs[] >>
+ res_tac >>
+ decide_tac,
+
+ rpt strip_tac >>
+ Cases_on ‘lookup_vexp scope_lists v’ >> (
+  fs[]
+ ) >>
+ Cases_on ‘bigstep_e_exec_l scope_lists e_l (n + 1)’ >> (
+  fs[]
+ ) >>
+ PairCases_on ‘x'’ >>
+ fs[] >>
+ res_tac >>
+ decide_tac,
+
+ rpt strip_tac >>
+ Cases_on ‘bigstep_e_exec_l scope_lists e_l n’ >> (
+  fs[]
+ ) >>
+ PairCases_on ‘x’ >>
+ fs[] >>
+ res_tac >>
+ decide_tac,
+
+ rpt strip_tac >>
+ Cases_on ‘bigstep_e_exec scope_lists h n’ >> (
+  fs[]
+ ) >>
+ PairCases_on ‘x’ >>
+ fs[] >>
+ Cases_on ‘is_v x0’ >> (
+  fs[]
+ ) >- (
+  Cases_on ‘e_exec_acc (e_acc x0 s)’ >> (
+   fs[]
+  ) >>
+  Cases_on ‘bigstep_e_exec_l scope_lists e_l (x1 + 1)’ >> (
+   fs[]
+  ) >>
+  PairCases_on ‘x'’ >>
+  fs[] >>
+  subgoal ‘x1 + 1 <= m’ >- (
+   cheat
+  ) >>
+  PAT_X_ASSUM “!e_l' scope_lists n m.
+          (case bigstep_e_exec scope_lists h n of
+             NONE => NONE
+           | SOME (h',n') =>
+             case bigstep_e_exec_l scope_lists e_l n' of
+               NONE => NONE
+             | SOME (t',n'') => SOME (h'::t',n'')) =
+          SOME (e_l',m) ==>
+          n <= m” (fn thm => ASSUME_TAC (Q.SPECL [‘x0::x'0’, ‘scope_lists’, ‘n’, ‘m’] thm)) >>
+  rfs[] >>
+  Cases_on ‘bigstep_e_exec_l scope_lists e_l x1’ >- (
+   (* Why can't this be NONE? *)
+   cheat
+  ) >>
+ PairCases_on ‘x'’ >>
+ fs[] >>
+ res_tac >>
+ rw[]
+
+  Cases_on ‘bigstep_e_exec_l scope_lists e_l (x1 + 1)’ >> (
+   fs[]
+  ) >>
+
+  res_tac >>
+  decide_tac
+ ) >>
+ res_tac >>
+ decide_tac
+
+
+cheat
+
+Induct_on ‘l’ >> (
+ rpt strip_tac >>
+ fs[bigstep_e_exec_def]
+) >>
+ Cases_on ‘bigstep_e_exec scope_lists (SND h) n’ >> (
+  fs[]
+ ) >>
+ PairCases_on ‘x’ >>
+ fs[] >>
+ Cases_on ‘bigstep_e_exec_l scope_lists (MAP SND l) x1’ >> (
+  fs[]
+ ) >>
+ PairCases_on ‘x’ >>
+ fs[] >>
+ PAT_X_ASSUM “!e. _” (fn thm => irule thm) >>
+
+ Cases_on ‘is_v x0’ >> Cases_on ‘EVERY is_v x0'’ >> (
+  fs[]
+ ) >>
+ qexistsl_tac [‘e_v (v_struct (ZIP (MAP FST l,vl_of_el (x0'))))’, ‘scope_lists’] >>
+*)
+QED
+ 
+Theorem bigstep_e_exec_incr:
+!e e' scope_lists n m.
+bigstep_e_exec scope_lists e n = SOME (e', m) ==>
+n <= m
+Proof
+Induct_on ‘e’ >> (
+ fs[bigstep_e_exec_def] >>
+ rpt strip_tac
+) >| [
+ Cases_on ‘lookup_vexp scope_lists v’ >>
+ fs[] >>
+ decide_tac,
+
+ bigstep_e_exec_case'_tac >>
+ Cases_on ‘is_v x0’ >> (
+  fs[]
+ ) >- (
+  Cases_on ‘e_exec_acc (e_acc x0 s)’ >> (
+   fs[]
+  ) >>
+  res_tac >>
+  decide_tac
+ ) >>
+ res_tac >>
+ decide_tac,
+
+ bigstep_e_exec_case'_tac >>
+ Cases_on ‘is_v x0’ >> (
+  fs[]
+ ) >- (
+  Cases_on ‘e_exec_unop u x0’ >> (
+   fs[]
+  ) >>
+  res_tac >>
+  decide_tac
+ ) >>
+ res_tac >>
+ decide_tac,
+
+ bigstep_e_exec_case'_tac >>
+ Cases_on ‘is_v x0’ >> (
+  fs[]
+ ) >- (
+  Cases_on ‘e_exec_cast c x0’ >> (
+   fs[]
+  ) >>
+  res_tac >>
+  decide_tac
+ ) >>
+ res_tac >>
+ decide_tac,
+
+ bigstep_e_exec_case'_tac >>
+ Cases_on ‘is_v x0’ >- (
+  Cases_on ‘x0’ >>
+  fs[is_v] >>
+  Cases_on ‘is_short_circuitable b’ >> (
+   fs[]
+  ) >- (
+   Cases_on ‘e_exec_short_circuit v b e'’ >> (
+    fs[]
+   ) >>
+   res_tac >>
+   decide_tac
+  ) >>
+  Cases_on ‘bigstep_e_exec scope_lists e' x1’ >> (
+   fs[]
+  ) >>
+  PairCases_on ‘x’ >>
+  fs[] >>
+  Cases_on ‘is_v x0’ >> (
+   fs[]
+  ) >- (
+   Cases_on ‘e_exec_binop (e_v v) b x0’ >> (
+    fs[]
+   ) >>
+   res_tac >>
+   decide_tac
+  ) >>
+  res_tac >>
+  decide_tac
+ ) >>
+ Cases_on ‘x0’ >> (
+  fs[is_v] >>
+  rw[] >>
+  res_tac >>
+  decide_tac
+ ),
+
+ (* Concat *)
+ bigstep_e_exec_case'_tac >>
+ Cases_on ‘is_v_bit x0’ >> (
+  fs[]
+ ) >- (
+  Cases_on ‘bigstep_e_exec scope_lists e' x1’ >> (
+   fs[]
+  ) >>
+  PairCases_on ‘x’ >>
+  fs[] >>
+  Cases_on ‘is_v_bit x0'’ >> (
+   fs[]
+  ) >- (
+   Cases_on ‘e_exec_concat x0 x0'’ >> (
+    fs[]
+   ) >>
+   res_tac >>
+   decide_tac
+  ) >>
+  res_tac >>
+  decide_tac
+ ) >>
+ res_tac >>
+ decide_tac,
+
+ bigstep_e_exec_case'_tac >>
+ Cases_on ‘is_v_bit x0’ >> (
+  fs[]
+ ) >- (
+  Cases_on ‘e_exec_slice x0 e' e''’ >> (
+   fs[]
+  ) >>
+  res_tac >>
+  decide_tac
+ ) >>
+ res_tac >>
+ decide_tac,
+
+ bigstep_e_exec_case'_tac >>
+ res_tac >>
+ decide_tac,
+
+ Cases_on ‘bigstep_e_exec_l scope_lists (MAP SND l) n’ >> (
+  fs[]
+ ) >>
+ PairCases_on ‘x’ >>
+ fs[] >>
+ Cases_on ‘EVERY is_v x0’ >> (
+  (* Need to be delicate here... *)
+  FULL_SIMP_TAC std_ss [] >>
+  fs[]
+ ) >> (
+  cheat
+ )
+]
+QED
+
+Theorem bigstep_e_exec_unchanged:
+!e e' scope_lists n.
+bigstep_e_exec scope_lists e n = SOME (e', n) ==>
+e = e'
+Proof
+cheat
+QED
+
+Theorem bigstep_e_exec_l_unchanged:
+!e_l e_l' scope_lists n.
+bigstep_e_exec_l scope_lists e_l n = SOME (e_l', n) ==>
+e_l = e_l'
+Proof
+cheat
+QED
+
+Theorem bigstep_e_exec_not_eq:
+!e e' scope_lists n.
+e <> e' ==>
+bigstep_e_exec scope_lists e 0 = SOME (e',n) ==>
+n <> 0
+Proof
+rpt strip_tac >>
+Cases_on ‘e’ >> (
+ fs[bigstep_e_exec_def]
+) >| [
+ Cases_on ‘lookup_vexp scope_lists v’ >>
+ fs[],
+
+ bigstep_e_exec_case_tac >>
+ Cases_on ‘is_v x0’ >> (
+  fs[]
+ ) >- (
+  Cases_on ‘e_exec_acc (e_acc x0 s)’ >> (
+   fs[]
+  )
+ ) >>
+ rw[] >>
+ imp_res_tac bigstep_e_exec_unchanged,
+
+ bigstep_e_exec_case_tac >>
+ Cases_on ‘is_v x0’ >> (
+  fs[]
+ ) >- (
+  Cases_on ‘e_exec_unop u x0’ >> (
+   fs[]
+  )
+ ) >>
+ rw[] >>
+ imp_res_tac bigstep_e_exec_unchanged,
+
+ bigstep_e_exec_case_tac >>
+ Cases_on ‘is_v x0’ >> (
+  fs[]
+ ) >- (
+  Cases_on ‘e_exec_cast c x0’ >> (
+   fs[]
+  )
+ ) >>
+ rw[] >>
+ imp_res_tac bigstep_e_exec_unchanged,
+
+ bigstep_e_exec_case_tac >>
+ Cases_on ‘is_v x0’ >- (
+  Cases_on ‘x0’ >>
+  fs[is_v] >>
+  Cases_on ‘is_short_circuitable b’ >> (
+   fs[]
+  ) >- (
+   Cases_on ‘e_exec_short_circuit v b e0’ >> (
+    fs[]
+   )
+  ) >>
+  Cases_on ‘bigstep_e_exec scope_lists e0 x1’ >> (
+   fs[]
+  ) >>
+  PairCases_on ‘x’ >>
+  fs[] >>
+  Cases_on ‘is_v x0’ >> (
+   fs[]
+  ) >- (
+   Cases_on ‘e_exec_binop (e_v v) b x0’ >> (
+    fs[]
+   )
+  ) >>
+  subgoal ‘x1 = 0’ >- (
+   rw[] >>
+   imp_res_tac bigstep_e_exec_incr >>
+   decide_tac
+  ) >>
+  rw[] >>
+  imp_res_tac bigstep_e_exec_unchanged >>
+  fs[]
+ ) >>
+ Cases_on ‘x0’ >>
+ fs[is_v] >> (
+  rw[] >>
+  imp_res_tac bigstep_e_exec_unchanged
+ ),
+
+ bigstep_e_exec_case_tac >>
+ Cases_on ‘is_v_bit x0’ >> (
+  fs[]
+ ) >- (
+  Cases_on ‘bigstep_e_exec scope_lists e0 x1’ >> (
+   fs[]
+  ) >>
+  PairCases_on ‘x’ >>
+  fs[] >>
+  Cases_on ‘is_v_bit x0'’ >> (
+   fs[]
+  ) >- (
+   Cases_on ‘e_exec_concat x0 x0'’ >> (
+    fs[]
+   )
+  ) >>
+  subgoal ‘x1 = 0’ >- (
+   rw[] >>
+   imp_res_tac bigstep_e_exec_incr >>
+   decide_tac
+  ) >>
+  rw[] >>
+  imp_res_tac bigstep_e_exec_unchanged >>
+  fs[]
+ ) >>
+ rw[] >>
+ imp_res_tac bigstep_e_exec_unchanged,
+
+ bigstep_e_exec_case_tac >>
+ Cases_on ‘is_v_bit x0’ >> (
+  fs[]
+ ) >- (
+  Cases_on ‘e_exec_slice x0 e0 e1’ >> (
+   fs[]
+  )
+ ) >>
+ rw[] >>
+ imp_res_tac bigstep_e_exec_unchanged,
+
+ bigstep_e_exec_case_tac >>
+ rw[] >>
+ imp_res_tac bigstep_e_exec_unchanged,
+
+ Cases_on ‘bigstep_e_exec_l scope_lists (MAP SND l) 0’ >> (
+  fs[]
+ ) >>
+ PairCases_on ‘x’ >>
+ fs[] >>
+ Cases_on ‘EVERY is_v x0’ >> (
+  (* Need to be delicate here... *)
+  FULL_SIMP_TAC std_ss []
+ ) >>
+ fs[] >>
+ rw[] >>
+ imp_res_tac bigstep_e_exec_l_unchanged >>
+ rw[] >>
+ fs[p4_auxTheory.ZIP_MAP_FST_SND]
+] 
+QED
+
+Theorem bigstep_e_exec_not_v_bit:
+!e e' scope_lists n.
+~is_v_bit e ==>
+is_v_bit e' ==>
+bigstep_e_exec scope_lists e 0 = SOME (e',n) ==>
+n <> 0
+Proof
+cheat
+QED
+
+Theorem bigstep_e_exec_not_v:
+!e e' scope_lists n.
+~is_v e ==>
+is_v e' ==>
+bigstep_e_exec scope_lists e 0 = SOME (e',n) ==>
+n <> 0
+Proof
+cheat
+(* OLD
+Induct_on ‘e’ >> (
+ fs[is_v]
+) >>
+rpt strip_tac >>
+Cases_on ‘e'’ >> (
+
+) >> 
+fs[is_v, bigstep_e_exec_def] >| [
+ Cases_on ‘lookup_vexp scope_lists v'’ >>
+ fs[],
+
+ bigstep_e_exec_case_tac >>
+ Cases_on ‘is_v x0’ >> (
+  fs[]
+ ) >>
+ Cases_on ‘e_exec_acc (e_acc x0 s)’ >> (
+  fs[]
+ ),
+
+ bigstep_e_exec_case_tac >>
+ Cases_on ‘is_v x0’ >> (
+  fs[]
+ ) >>
+ Cases_on ‘e_exec_unop u x0’ >> (
+  fs[]
+ ),
+
+ bigstep_e_exec_case_tac >>
+ Cases_on ‘is_v x0’ >> (
+  fs[]
+ ) >>
+ Cases_on ‘e_exec_cast c x0’ >> (
+  fs[]
+ ),
+
+ bigstep_e_exec_case_tac >>
+ Cases_on ‘is_v x0’ >> (
+  Cases_on ‘x0’ >>
+  fs[is_v]
+ ) >>
+ Cases_on ‘is_short_circuitable b’ >> (
+  fs[]
+ ) >- (
+  Cases_on ‘e_exec_short_circuit v' b e0’ >> (
+   fs[]
+  )
+ ) >>
+ Cases_on ‘bigstep_e_exec scope_lists e0 x1’ >> (
+  fs[]
+ ) >>
+ PairCases_on ‘x’ >>
+ fs[] >>
+ Cases_on ‘is_v x0’ >> (
+  Cases_on ‘x0’ >>
+  fs[is_v]
+ ) >>
+ Cases_on ‘e_exec_binop (e_v v') b (e_v v'')’ >> (
+  fs[]
+ ),
+
+ bigstep_e_exec_case_tac >>
+ Cases_on ‘is_v_bit x0’ >> (
+  fs[]
+ ) >>
+ Cases_on ‘bigstep_e_exec scope_lists e0 x1’ >> (
+  fs[]
+ ) >>
+ PairCases_on ‘x’ >>
+ fs[] >>
+ Cases_on ‘is_v_bit x0'’ >> (
+  fs[]
+ ) >>
+ Cases_on ‘e_exec_concat x0 x0'’ >> (
+  fs[]
+ ),
+
+ bigstep_e_exec_case_tac >>
+ Cases_on ‘is_v_bit x0’ >> (
+  fs[]
+ ) >>
+ Cases_on ‘e_exec_slice x0 e0 e1’ >> (
+  fs[]
+ ),
+
+ bigstep_e_exec_case_tac,
+
+ Cases_on ‘bigstep_e_exec_l scope_lists (MAP SND l) 0’ >> (
+  fs[]
+ ) >>
+ PairCases_on ‘x’ >>
+ fs[] >>
+ Cases_on ‘EVERY is_v x0’ >> (
+  (* Need to be delicate here... *)
+  FULL_SIMP_TAC std_ss []
+ ) >>
+ fs[]
+]
+*)
+QED
+
+
+fun bigstep_e_exec_sound_single_rec_tac tmq1 tmq2 =
+ Cases_on ‘is_v e’ >> (
+  fs[]
+ ) >- (
+  (* Base case *)
+  Cases_on ‘e’ >> (
+   fs[is_v, bigstep_e_exec_def]
+  ) >>
+  Cases_on tmq1 >> (
+   fs[]
+  )
+ ) >>
+ (* Recursive case *)
+ Cases_on ‘bigstep_e_exec (scope_list ++ g_scope_list') e 0’ >> (
+  fs[]
+ ) >>
+ PairCases_on ‘x’ >>
+ fs[] >>
+ Cases_on ‘is_v x0’ >> (
+  fs[]
+ ) >| [
+  Cases_on tmq2 >> (
+   fs[]
+  ) >>
+  imp_res_tac bigstep_e_exec_not_v,
+
+  rfs[] >>
+  res_tac >>
+  fs[]
+ ]
+;
+
+
+Theorem bigstep_e_exec_v:
+!v scope_list g_scope_list' n.
+bigstep_e_exec (scope_list ++ g_scope_list') (e_v v) n = SOME (e_v v, n)
+Proof
+cheat
+QED
+
+Theorem bigstep_e_exec_l_all_red:
+!e_l scope_lists n.
+unred_mem_index e_l = NONE ==>
+bigstep_e_exec_l scope_lists e_l n = SOME (e_l,n+1)
+Proof
+cheat
+QED
+
+Theorem bigstep_e_exec_l_single_unred:
+!e_l e_l' e' x scope_lists n.
+unred_mem_index e_l = SOME x ==>
+bigstep_e_exec_l scope_lists e_l n = SOME (e_l',n+1) ==>
+bigstep_e_exec scope_lists (EL x e_l) n = SOME (e', n+1) /\ e_l' = LUPDATE e' x e_l
+Proof
+cheat
+QED
+
+Theorem bigstep_e_exec_sound:
+!e scope_list g_scope_list' e' apply_table_f (ext_map:'a ext_map) func_map b_func_map pars_map tbl_map.
+bigstep_e_exec (scope_list ++ g_scope_list') e 0 = SOME (e', 1) ==>
+e_exec (apply_table_f,ext_map,func_map,b_func_map,pars_map,tbl_map)
+             g_scope_list' scope_list e = SOME (e', [])
+Proof
+Induct_on ‘e’ >> (
+ rpt strip_tac >>
+ fs[bigstep_e_exec_def, e_exec]
+) >| [
+ (* var *)
+ fs[lookup_vexp_def, lookup_vexp2_def] >>
+ Cases_on ‘lookup_map (scope_list ++ g_scope_list') v’ >> (
+  fs[]
+ ) >>
+ Cases_on ‘x’ >> (
+  fs[]
+ ),
+
+ (* acc *)
+ (*
+  val tmq1 = ‘e_exec_acc (e_acc (e_v v) s)’
+  val tmq2 = ‘e_exec_acc (e_acc x0 s)’
+ *)
+ bigstep_e_exec_sound_single_rec_tac ‘e_exec_acc (e_acc (e_v v) s)’ ‘e_exec_acc (e_acc x0 s)’,
+
+ (* Unop *)
+ bigstep_e_exec_sound_single_rec_tac ‘e_exec_unop u (e_v v)’ ‘e_exec_unop u x0’,
+
+ (* Cast *)
+ bigstep_e_exec_sound_single_rec_tac ‘e_exec_cast c (e_v v)’ ‘e_exec_cast c x0’,
+
+ (* Binop *)
+ Cases_on ‘bigstep_e_exec (scope_list ++ g_scope_list') e 0’ >> (
+  fs[]
+ ) >>
+ PairCases_on ‘x’ >>
+ fs[] >>
+ Cases_on ‘is_v e’ >- (
+  Cases_on ‘e’ >> (
+   fs[is_v]
+  ) >>
+  subgoal ‘x0 = e_v v /\ x1 = 0’ >- (
+   fs[bigstep_e_exec_v]
+  ) >>
+  gs[] >>
+  Cases_on ‘is_short_circuitable b’ >> (
+   fs[]
+  ) >- (
+   Cases_on ‘e_exec_short_circuit v b e'’ >> (
+    fs[]
+   )
+  ) >>
+  Cases_on ‘bigstep_e_exec (scope_list ++ g_scope_list') e' 0’ >> (
+   fs[]
+  ) >>
+  PairCases_on ‘x’ >>
+  fs[] >>
+  Cases_on ‘is_v e'’ >> (
+   fs[]
+  ) >- (
+   (* Second operand not reduced *)
+   rw[] >>
+   Cases_on ‘e'’ >> (
+    fs[is_v]
+   ) >>
+   subgoal ‘x0' = e_v v' /\ x1' = 0’ >- (
+    fs[bigstep_e_exec_v]
+   ) >>
+   fs[is_v] >>
+   Cases_on ‘e_exec_binop (e_v v) b (e_v v')’ >> (
+    fs[]
+   )
+  ) >>
+  Cases_on ‘is_v x0'’ >> (
+   fs[]
+  ) >- (
+   (* Contradiction on n *)
+   imp_res_tac bigstep_e_exec_not_v >>
+   Cases_on ‘e_exec_binop (e_v v) b x0'’ >> (
+    fs[]
+   )
+  ) >>
+  (* Inductive case *)
+  gs[] >>
+  res_tac >>
+  fs[] >>
+  Cases_on ‘e’ >> (
+   fs[is_v_bit, bigstep_e_exec_def]
+  )
+ ) >>
+ (* Second operand *)
+ Cases_on ‘is_v x0’ >> (
+  fs[]
+ ) >- (
+  Cases_on ‘x0’ >> (
+   fs[is_v]
+  ) >>
+  subgoal ‘x1 = 1’ >- (
+   subgoal ‘is_v $ e_v v’ >- (
+    fs[is_v]
+   ) >>
+   imp_res_tac bigstep_e_exec_not_v >>
+   Cases_on ‘bigstep_e_exec (scope_list ++ g_scope_list') e' x1’ >> (
+    fs[]
+   ) >- (
+    Cases_on ‘e_exec_short_circuit v b e'’ >> (
+     fs[]
+    )
+   ) >>
+   PairCases_on ‘x’ >>
+   fs[] >>
+   Cases_on ‘is_short_circuitable b’ >> (
+    fs[]
+   ) >- (
+    Cases_on ‘e_exec_short_circuit v b e'’ >> (
+     fs[]
+    )
+   ) >>
+   Cases_on ‘is_v x0’ >> (
+    fs[]
+   ) >- (
+    Cases_on ‘e_exec_binop (e_v v) b x0’ >> (
+     fs[]
+    ) >>
+    imp_res_tac bigstep_e_exec_incr >>
+    decide_tac
+   ) >>
+   imp_res_tac bigstep_e_exec_incr >>
+   decide_tac
+  ) >>
+  fs[] >>
+  Cases_on ‘bigstep_e_exec (scope_list ++ g_scope_list') e' 1’ >> (
+   fs[]
+  ) >- (
+   Cases_on ‘e_exec_short_circuit v b e'’ >> (
+    fs[]
+   )
+  ) >>
+  Cases_on ‘is_short_circuitable b’ >> (
+   fs[]
+  ) >- (
+   Cases_on ‘e_exec_short_circuit v b e'’ >> (
+    fs[]
+   )
+  ) >>
+  PairCases_on ‘x’ >>
+  fs[] >>
+  subgoal ‘~is_v x0’ >- (
+   CCONTR_TAC >>
+   fs[] >>
+   Cases_on ‘e_exec_binop (e_v v) b x0’ >> (
+    fs[]
+   ) >>
+   imp_res_tac bigstep_e_exec_incr >>
+   decide_tac
+  ) >>
+  gs[] >>
+  res_tac >>
+  fs[] >>
+  subgoal ‘e' = x0’ >- (
+   imp_res_tac bigstep_e_exec_unchanged
+  ) >>
+  Cases_on ‘e’ >> (
+   fs[is_v, bigstep_e_exec_def]
+  )
+ ) >>
+ Cases_on ‘x0’ >> Cases_on ‘e’ >> (
+  fs[is_v, bigstep_e_exec_def] >>
+  gs[] >>
+  res_tac >>
+  fs[]
+ ),
+
+ (* Concat *)
+ Cases_on ‘bigstep_e_exec (scope_list ++ g_scope_list') e 0’ >> (
+  fs[]
+ ) >>
+ PairCases_on ‘x’ >>
+ fs[] >>
+ Cases_on ‘is_v_bit e’ >> (
+  fs[]
+ ) >- (
+  Cases_on ‘e’ >> (
+   fs[is_v_bit]
+  ) >>
+  (* First operand not reduced *)
+  subgoal ‘x0 = e_v v /\ x1 = 0’ >- (
+   fs[bigstep_e_exec_v]
+  ) >>
+  fs[] >>
+  Cases_on ‘bigstep_e_exec (scope_list ++ g_scope_list') e' 0’ >> (
+   fs[]
+  ) >>
+  PairCases_on ‘x’ >>
+  fs[] >>
+  Cases_on ‘is_v_bit e'’ >> (
+   fs[]
+  ) >- (
+   (* Second operand not reduced *)
+   rw[] >>
+   Cases_on ‘e'’ >> (
+    fs[is_v_bit]
+   ) >>
+   subgoal ‘x0' = e_v v' /\ x1' = 0’ >- (
+    fs[bigstep_e_exec_v]
+   ) >>
+   fs[] >>
+   Cases_on ‘v’ >> (
+    gvs[is_v_bit]
+   ) >>
+   Cases_on ‘v'’ >> (
+    gvs[is_v_bit]
+   ) >>
+   Cases_on ‘e_exec_concat (e_v (v_bit p)) (e_v (v_bit p'))’ >> (
+    fs[]
+   )
+  ) >>
+  (* Second operand was reduced, or e subtype contradiction *)
+  Cases_on ‘is_v_bit x0'’ >> (
+   fs[]
+  ) >- (
+   (* Contradiction on n *)
+   Cases_on ‘x0'’ >> (
+    fs[is_v_bit]
+   ) >>
+   imp_res_tac bigstep_e_exec_not_v_bit >>
+   Cases_on ‘e_exec_concat (e_v v) (e_v v')’ >> (
+    fs[]
+   )
+  ) >>
+  (* Inductive case *)
+  gs[] >>
+  res_tac >>
+  fs[] >>
+  Cases_on ‘e’ >> (
+   fs[is_v_bit, bigstep_e_exec_def]
+  )
+ ) >>
+ (* First operand was reduced *)
+ Cases_on ‘is_v_bit x0’ >> (
+  fs[]
+ ) >- (
+  subgoal ‘x1 = 1’ >- (
+   imp_res_tac bigstep_e_exec_not_v_bit >>
+   Cases_on ‘bigstep_e_exec (scope_list ++ g_scope_list') e' x1’ >> (
+    fs[]
+   ) >>
+   PairCases_on ‘x’ >>
+   fs[] >>
+   Cases_on ‘is_v_bit x0'’ >> (
+    fs[]
+   ) >- (
+    Cases_on ‘e_exec_concat x0 x0'’ >> (
+     fs[]
+    ) >>
+    imp_res_tac bigstep_e_exec_incr >>
+    decide_tac
+   ) >>
+   imp_res_tac bigstep_e_exec_incr >>
+   decide_tac
+  ) >>
+  fs[] >>
+  Cases_on ‘bigstep_e_exec (scope_list ++ g_scope_list') e' 1’ >> (
+   fs[]
+  ) >>
+  PairCases_on ‘x’ >>
+  fs[] >>
+  subgoal ‘~is_v_bit x0'’ >- (
+   CCONTR_TAC >>
+   fs[] >>
+   Cases_on ‘e_exec_concat x0 x0'’ >> (
+    fs[]
+   ) >>
+   imp_res_tac bigstep_e_exec_incr >>
+   decide_tac
+  ) >>
+  fs[] >>
+  gs[] >>
+  res_tac >>
+  fs[] >>
+  subgoal ‘e' = x0'’ >- (
+   imp_res_tac bigstep_e_exec_unchanged
+  ) >>
+  fs[]
+ ) >>
+ (* Inductive case *)
+ gs[] >>
+ res_tac >>
+ fs[] >>
+ Cases_on ‘e’ >> (
+  fs[is_v_bit, bigstep_e_exec_def]
+ ),
+
+ (* Slice *)
+ Cases_on ‘bigstep_e_exec (scope_list ++ g_scope_list') e 0’ >> (
+  fs[]
+ ) >>
+ PairCases_on ‘x’ >>
+ fs[] >>
+ Cases_on ‘is_v_bit e’ >> (
+  fs[]
+ ) >- (
+  Cases_on ‘e’ >> (
+   fs[is_v_bit]
+  ) >>
+  subgoal ‘x0 = e_v v /\ x1 = 0’ >- (
+   fs[bigstep_e_exec_v]
+  ) >>
+  fs[] >>
+  Cases_on ‘e_exec_slice (e_v v) e' e''’ >> (
+   fs[]
+  )
+ ) >>
+ subgoal ‘~is_v_bit x0’ >> (
+  CCONTR_TAC >>
+  fs[] >>
+  Cases_on ‘e_exec_slice x0 e' e''’ >> (
+   fs[]
+  ) >>
+  rfs[] >>
+  imp_res_tac bigstep_e_exec_unchanged >>
+  fs[is_v_bit]
+ ) >>
+ gs[] >>
+ res_tac >>
+ fs[],
+
+ (* Select *)
+ Cases_on ‘bigstep_e_exec (scope_list ++ g_scope_list') e 0’ >> (
+  fs[]
+ ) >>
+ PairCases_on ‘x’ >>
+ fs[] >>
+ Cases_on ‘is_v e’ >> (
+  fs[]
+ ) >- (
+  Cases_on ‘e’ >> (
+   fs[is_v]
+  ) >>
+  fs[bigstep_e_exec_v]
+ ) >>
+ gs[] >>
+ res_tac >>
+ fs[],
+
+ (* Struct entry *)
+(* OLD
+ Induct_on ‘l’ >> (
+  fs[bigstep_e_exec_def]
+ ) >- (
+  fs[unred_mem_index_def, unred_mem_def, listTheory.INDEX_FIND_def]
+ ) >>
+*)
+ rpt strip_tac >>
+ Cases_on ‘unred_mem_index (MAP SND l)’ >> (
+  fs[]
+ ) >- (
+  imp_res_tac bigstep_e_exec_l_all_red >>
+  Cases_on ‘bigstep_e_exec_l (scope_list ++ g_scope_list') (MAP SND l) 0’ >> (
+   fs[]
+  ) >>
+  PairCases_on ‘x’ >>
+  fs[] >>
+  subgoal ‘EVERY is_v x0’ >- (
+   cheat
+  ) >>
+  fs[] >>
+  gvs[]
+ ) >>
+ Cases_on ‘bigstep_e_exec_l (scope_list ++ g_scope_list') (MAP SND l) 0’ >> (
+  fs[]
+ ) >>
+ PairCases_on ‘x'’ >>
+ fs[] >>
+ subgoal ‘~EVERY is_v x'0’ >- (
+  cheat
+ ) >>
+ FULL_SIMP_TAC std_ss [] >>
+ rw[] >>
+ imp_res_tac bigstep_e_exec_l_single_unred >>
+ (* TODO: This requires some further thought... *)
+ cheat
+]
+QED
+
+Theorem scope_lists_separate:
+!scope_lists top_scope scope_list scope_list' g_scope_list' g_scope_list''.
+scope_lists = top_scope::(scope_list ++ g_scope_list') ==>
+           separate scope_lists = (SOME g_scope_list'',SOME scope_list') ==>
+           g_scope_list' = g_scope_list'' /\ top_scope::scope_list = scope_list'
+Proof
+rpt gen_tac >> rpt disch_tac >>
+subgoal ‘LENGTH g_scope_list' = 2’ >- (
+ cheat
+) >>
+rpt strip_tac >> (
+ rw[]
+) >>
+fs[separate_def] >>
+gs[arithmeticTheory.ADD_SUC] >>
+FULL_SIMP_TAC pure_ss [GSYM SUC_ADD_ONE] >>
+fs[oDROP_def, oTAKE_def, oDROP_APPEND, oTAKE_APPEND]
+QED
+
+(* TODO: Prove where that arch_frame_list_regular is obtained for all SOME results? *)
+Theorem bigstep_stmt_exec_sound:
+!h scope_list g_scope_list' g_scope_list''
+stmt' scope_lists scope_list' funn t top_scope apply_table_f ext_map func_map x' pars_map x'' ascope.
+bigstep_stmt_exec (NONE:(func_map # b_func_map # 'a ext_map) option) ((top_scope::scope_list)++g_scope_list') h 0 = SOME (stmt', scope_lists, 1) ==>
+separate scope_lists = (SOME g_scope_list'',SOME scope_list') ==>
+stmt_exec (apply_table_f,ext_map:'a ext_map,func_map,x',pars_map,x'')
+             (ascope,g_scope_list',[(funn,h::t,(top_scope::scope_list))],status_running) = SOME (ascope, g_scope_list'', [(funn,stmt'::t,scope_list')], status_running)
+Proof
+Induct_on ‘h’ >> (
+ rpt strip_tac
+) >| [
+ (* empty *)
+ fs[bigstep_stmt_exec_def],
+
+ (* assign *)
+ Cases_on ‘t’ >> (
+  fs[stmt_exec]
+ ) >> (
+ (* Both cases of t identical *)
+  Cases_on ‘is_v e’ >> (
+   fs[]
+  ) >- (
+   Cases_on ‘e’ >> (
+    fs[is_v]
+   ) >>
+   fs[bigstep_stmt_exec_def, bigstep_e_exec_def, is_v] >>
+   Cases_on ‘stmt_exec_ass l (e_v v) (top_scope::(scope_list ++ g_scope_list'))’ >> (
+    fs[]
+   )
+  ) >>
+  (* e reduction *)
+  fs[bigstep_stmt_exec_def] >>
+  Cases_on ‘?funn' e_l. e = e_call funn e_l’ >> (
+   gs[bigstep_f_arg_exec_def]
+  ) >>
+  Cases_on ‘bigstep_e_exec (top_scope::(scope_list ++ g_scope_list')) e 0’ >> (
+   fs[]
+  ) >- (
+   Cases_on ‘e’ >> (
+    fs[]
+   )
+  ) >>
+  PairCases_on ‘x’ >>
+  fs[] >>
+  subgoal ‘x1 = 1’ >- (
+   cheat
+  ) >>
+  fs[] >>
+  FULL_SIMP_TAC pure_ss [GSYM listTheory.APPEND] >>
+  imp_res_tac bigstep_e_exec_sound >>
+  fs[] >>
+  Cases_on ‘e’ >> (
+   fs[]
+  ) >> (
+   (* All different cases of e *)
+   Cases_on ‘is_v x0’ >> (
+    fs[]
+   ) >- (
+    Cases_on ‘stmt_exec_ass l x0 (top_scope::(scope_list ++ g_scope_list'))’ >> (
+     fs[]
+    )
+   ) >>
+   irule scope_lists_separate >>
+   metis_tac[]
+  )
+ ),
+
+ (* Conditional *)
+ Cases_on ‘t’ >> (
+  fs[stmt_exec]
+ ) >> (
+  Cases_on ‘is_v_bool e’ >> (
+   fs[]
+  ) >- (
+   Cases_on ‘e’ >> (
+    fs[is_v_bool]
+   ) >>
+   Cases_on ‘v’ >> (
+    fs[is_v_bool]
+   ) >>
+   fs[bigstep_stmt_exec_def, bigstep_e_exec_def]
+  ) >>
+  (* e reduction *)
+  fs[bigstep_stmt_exec_def] >>
+  Cases_on ‘?funn' e_l. e = e_call funn e_l’ >> (
+   gs[bigstep_f_arg_exec_def]
+  ) >>
+  Cases_on ‘bigstep_e_exec (top_scope::(scope_list ++ g_scope_list')) e 0’ >> (
+   fs[]
+  ) >- (
+   Cases_on ‘e’ >> (
+    fs[]
+   )
+  ) >>
+  PairCases_on ‘x’ >>
+  fs[] >>
+  subgoal ‘x1 = 1’ >- (
+   cheat
+  ) >>
+  fs[] >>
+  FULL_SIMP_TAC pure_ss [GSYM listTheory.APPEND] >>
+  imp_res_tac bigstep_e_exec_sound >>
+  fs[] >>
+  Cases_on ‘e’ >> (
+   fs[]
+  ) >> (
+   (* All different cases of e *)
+   irule scope_lists_separate >>
+   metis_tac[]
+  )
+ ),
+ 
+ (* block *)
+ fs[bigstep_stmt_exec_def],
+
+ (* return *)
+ Cases_on ‘t’ >> (
+  fs[stmt_exec]
+ ) >> (
+  Cases_on ‘get_v e <> NONE’ >> (
+   fs[]
+  ) >- (
+   subgoal ‘?x. get_v e = SOME x’ >- (
+    fs[GSYM quantHeuristicsTheory.IS_SOME_EQ_NOT_NONE, optionTheory.IS_SOME_EXISTS]
+   ) >>
+   Cases_on ‘e’ >> (
+    fs[get_v]
+   ) >>
+   fs[bigstep_stmt_exec_def, bigstep_e_exec_def]
+  ) >>
+  (* e reduction *)
+  fs[bigstep_stmt_exec_def] >>
+  Cases_on ‘bigstep_e_exec (top_scope::(scope_list ++ g_scope_list')) e 0’ >> (
+   fs[]
+  ) >>
+  PairCases_on ‘x’ >>
+  gs[] >>
+  rw[] >>
+  FULL_SIMP_TAC pure_ss [GSYM listTheory.APPEND] >>
+  imp_res_tac bigstep_e_exec_sound >>
+  fs[] >>
+  irule scope_lists_separate >>
+  metis_tac[]
+ ),
+
+ (* seq - recursive case *)
+ cheat,
+
+ (* transition *)
+ Cases_on ‘t’ >> (
+  fs[stmt_exec]
+ ) >> (
+  Cases_on ‘is_v e’ >> (
+   fs[]
+  ) >- (
+   Cases_on ‘is_v_str e’ >> (
+    fs[]
+   ) >> (
+    Cases_on ‘e’ >> (
+     fs[is_v, is_v_str]
+    ) >>
+    Cases_on ‘v’ >> (
+     fs[is_v, is_v_str]
+    ) >>
+    fs[bigstep_stmt_exec_def, bigstep_e_exec_def]
+   )
+  ) >>
+  (* e reduction *)
+  fs[bigstep_stmt_exec_def] >>
+  Cases_on ‘bigstep_e_exec (top_scope::(scope_list ++ g_scope_list')) e 0’ >> (
+   fs[]
+  ) >>
+  PairCases_on ‘x’ >>
+  gs[] >>
+  rw[] >>
+  FULL_SIMP_TAC pure_ss [GSYM listTheory.APPEND] >>
+  imp_res_tac bigstep_e_exec_sound >>
+  fs[] >>
+  irule scope_lists_separate >>
+  metis_tac[]
+ ),
+
+ (* apply *)
+ Cases_on ‘t’ >> (
+  fs[stmt_exec]
+ ) >> (
+  Cases_on ‘index_not_const l’ >> (
+   fs[]
+  ) >- (
+   (* Contradiction on l being reduced, while index_not_const l = NONE *)
+   cheat
+  ) >>
+  (* e reduction *)
+  fs[bigstep_stmt_exec_def] >>
+  Cases_on ‘bigstep_e_exec_l (top_scope::(scope_list ++ g_scope_list')) l 0’ >> (
+   fs[]
+  ) >>
+  PairCases_on ‘x'3'’ >>
+  gs[] >>
+  rw[] >>
+  FULL_SIMP_TAC pure_ss [GSYM listTheory.APPEND] >>
+  cheat
+(*
+  imp_res_tac bigstep_e_exec_l_sound >>
+  fs[] >>
+  irule scope_lists_separate >>
+  metis_tac[]
+*)
+ ),
+
+ (* ext *)
+ fs[bigstep_stmt_exec_def]
+]
+QED
+
+Theorem bigstep_arch_exec_sound_NONE_1:
+!i ab_list x el pblock_map pbl_type x_d_list b_func_map decl_list pars_map tbl_map funn stmt_stack scope_list top_scope frame_list func_map in_out_list in_out_list' ascope g_scope_list g_scope_list' g_scope_list'' arch_frame_list' g_scope_list''' ffblock_map input_f output_f copyin_pbl copyout_pbl apply_table_f ext_map.
+(EL i ab_list = (arch_block_pbl x el)) ==>
+(ALOOKUP pblock_map x = SOME (pbl_type, x_d_list, b_func_map, decl_list, pars_map, tbl_map)) ==>
+~(state_fin_exec status_running ((funn, stmt_stack, (top_scope::scope_list))::frame_list)) ==>
+scopes_to_pass funn func_map b_func_map g_scope_list = SOME g_scope_list' ==>
+map_to_pass funn b_func_map <> NONE ==>
+tbl_to_pass funn b_func_map tbl_map <> NONE ==>
+bigstep_arch_exec (NONE:('a actx # b_func_map) option) (g_scope_list':g_scope_list) (arch_frame_list_regular ((funn, stmt_stack, (top_scope::scope_list))::frame_list)) = SOME (g_scope_list'', arch_frame_list', 1) ==>
+scopes_to_retrieve funn func_map b_func_map g_scope_list g_scope_list'' = SOME g_scope_list''' ==>
+arch_exec ((ab_list, pblock_map, ffblock_map, input_f, output_f, copyin_pbl, copyout_pbl, apply_table_f, ext_map, func_map):'a actx) ((i, in_out_list, in_out_list', ascope), g_scope_list, (arch_frame_list_regular ((funn, stmt_stack, (top_scope::scope_list))::frame_list)), status_running) = SOME ((i, in_out_list, in_out_list', ascope), g_scope_list''', arch_frame_list', status_running)
+Proof
+fs [arch_exec_def] >>
+rpt strip_tac >>
+fs [state_fin_exec_equiv, state_fin_def] >>
+Cases_on ‘map_to_pass funn b_func_map’ >> (
+ fs[]
+) >>
+Cases_on ‘tbl_to_pass funn b_func_map tbl_map’ >> (
+ fs[]
+) >>
+fs[bigstep_arch_exec_def] >>
+Cases_on ‘stmt_stack’ >> (
+ fs[]
+) >>
+fs[bigstep_exec_def] >>
+Cases_on ‘bigstep_stmt_exec NONE ((top_scope::scope_list) ++ g_scope_list') h 0’ >> (
+ fs[]
+) >>
+PairCases_on ‘x'3'’ >>
+fs[] >>
+Cases_on ‘separate x'''1’ >> (
+ fs[]
+) >>
+Cases_on ‘q’ >> (
+ fs[]
+) >>
+Cases_on ‘r’ >> (
+ fs[]
+) >>
+rw[] >>
+Cases_on `frames_exec
+           (apply_table_f,ext_map,func_map,b_func_map,pars_map,tbl_map)
+           (ascope,g_scope_list,(funn,stmt_stack,(top_scope::scope_list))::frame_list,
+            status_running)` >> (
+ fs []
+) >- (
+ fs[bigstep_arch_exec_def] >>
+ Cases_on ‘frame_list’ >> (
+  fs[bigstep_exec_def, frames_exec]
+ ) >| [
+  ALL_TAC,
+
+  PairCases_on ‘h'’ >>
+  fs[bigstep_exec_def, frames_exec]
+ ] >> (
+  FULL_SIMP_TAC pure_ss [GSYM listTheory.APPEND] >>
+  imp_res_tac bigstep_stmt_exec_sound >>
+  gs[]
+ )
+) >>
+PairCases_on ‘x'3'’ >>
+fs[bigstep_arch_exec_def] >>
+Cases_on ‘frame_list’ >> (
+ fs[bigstep_exec_def, frames_exec]
+) >| [
+ ALL_TAC,
+
+ PairCases_on ‘h'’ >>
+ fs[bigstep_exec_def, frames_exec]
+] >> (
+ FULL_SIMP_TAC pure_ss [GSYM listTheory.APPEND] >>
+ imp_res_tac bigstep_stmt_exec_sound >>
+ gs[] >> (
+  FULL_SIMP_TAC pure_ss [GSYM listTheory.APPEND] >>
+  imp_res_tac bigstep_stmt_exec_sound >>
+  gs[]
+ )
+)
+QED
 
 Theorem bigstep_arch_exec_sound_NONE:
-!i ab_list x el pblock_map pbl_type x_d_list b_func_map decl_list pars_map tbl_map funn stmt_stack scope_list frame_list func_map g_scope_list g_scope_list' g_scope_list'' arch_frame_list' n g_scope_list''' ffblock_map input_f output_f copyin_pbl copyout_pbl apply_table_f ext_map aenv.
+!i ab_list x el pblock_map pbl_type x_d_list b_func_map decl_list pars_map tbl_map funn stmt_stack scope_list frame_list func_map in_out_list in_out_list' ascope g_scope_list g_scope_list' g_scope_list'' arch_frame_list' n g_scope_list''' ffblock_map input_f output_f copyin_pbl copyout_pbl apply_table_f ext_map.
 (EL i ab_list = (arch_block_pbl x el)) ==>
 (ALOOKUP pblock_map x = SOME (pbl_type, x_d_list, b_func_map, decl_list, pars_map, tbl_map)) ==>
 ~(state_fin_exec status_running ((funn, stmt_stack, scope_list)::frame_list)) ==>
@@ -354,7 +1688,7 @@ map_to_pass funn b_func_map <> NONE ==>
 tbl_to_pass funn b_func_map tbl_map <> NONE ==>
 bigstep_arch_exec NONE (g_scope_list':g_scope_list) (arch_frame_list_regular ((funn, stmt_stack, scope_list)::frame_list)) = SOME (g_scope_list'', arch_frame_list', n) ==>
 scopes_to_retrieve funn func_map b_func_map g_scope_list g_scope_list'' = SOME g_scope_list''' ==>
-arch_multi_exec ((ab_list, pblock_map, ffblock_map, input_f, output_f, copyin_pbl, copyout_pbl, apply_table_f, ext_map, func_map):'a actx) (aenv, g_scope_list, (arch_frame_list_regular ((funn, stmt_stack, scope_list)::frame_list)), status_running) n = SOME (aenv, g_scope_list''', arch_frame_list', status_running)
+arch_multi_exec ((ab_list, pblock_map, ffblock_map, input_f, output_f, copyin_pbl, copyout_pbl, apply_table_f, ext_map, func_map):'a actx) ((i, in_out_list, in_out_list', ascope), g_scope_list, (arch_frame_list_regular ((funn, stmt_stack, scope_list)::frame_list)), status_running) n = SOME ((i, in_out_list, in_out_list', ascope), g_scope_list''', arch_frame_list', status_running)
 Proof
 cheat
 QED
